lib/Lib.ByteSequence.fsti
@@ -174,3 +174,6 @@ val lemma_nat_from_to_bytes_le_preserves_value: #l:secrecy_level -> b:bytes_l l 
   Lemma
   (requires (True))
   (ensures  (nat_to_bytes_le #l len (nat_from_bytes_le b)) == b)
+
+val lemma_reveal_uint_to_bytes_le: #t:inttype{t <> U1} -> #l:secrecy_level -> b:bytes_l l{Lib.Sequence.length b == numbytes t} ->
+  Lemma (nat_from_bytes_le b == uint_v (uint_from_bytes_le #t #l b))
